

**School Of Engineering,  
Dayananda Sagar University,  
3rd Sem  
Module 3 : Fourier Transform**

Fourier Series is used for functions that are periodic on a finite interval only. When the functions are non-periodic and are defined on the whole x-axis, this concept is extended and it leads to Fourier integrals.

## 1 Fourier Integral

If  $f(x)$  is a piecewise continuous function with right and left hand derivative at every point and if it is absolutely integrable on the x-axis, then The fourier integral is given by

$$\boxed{f(x) = \int_0^{\infty} [A(\omega)\cos\omega x + B(\omega)\sin\omega x]d\omega} \quad (1.1)$$

where  $A(\omega) = \frac{1}{\pi} \int_{-\infty}^{\infty} f(v)\cos(\omega v)dv$  and  $B(\omega) = \frac{1}{\pi} \int_{-\infty}^{\infty} f(v)\sin(\omega v)dv$ .

**Ques 1.** Find the fourier integral representation of  $f(x) = \begin{cases} 1, & \text{if } |x| < 1 \\ 0, & \text{if } |x| > 1 \end{cases}$ .

**Soln.**  $A(\omega) = \frac{1}{\pi} \int_{-\infty}^{\infty} f(v)\cos(\omega v)dv$   
cos is an even function.

$$\begin{aligned} A(\omega) &= \frac{1}{\pi} \int_{-1}^1 \cos(\omega v)dv \\ &= \frac{2}{\pi} \int_0^1 \cos(\omega v)dv \\ &= \frac{2}{\pi} \left[ \frac{\sin(\omega v)}{\omega} \right]_0^1 \\ &= \frac{2}{\pi} \left[ \frac{\sin(\omega)}{\omega} \right] \end{aligned}$$

$$B(\omega) = \frac{1}{\pi} \int_{-\infty}^{\infty} f(v)\sin(\omega v)dv.$$

$$B(\omega) = \frac{1}{\pi} \int_{-1}^1 f(v)\sin(\omega v)dv = 0,$$

since  $\sin$  is an odd function.

Thus,

$$\begin{aligned} f(x) &= \int_0^\infty [A(\omega)\cos\omega x + B(\omega)\sin\omega x]d\omega \\ &= \int_0^\infty \frac{2}{\pi} \left[ \frac{\sin(\omega)}{\omega} \right] \cos(\omega x) d\omega \end{aligned}$$

## 2 Complex Form of Fourier Integral

The fourier integral is given by

$$\boxed{f(x) = \int_0^\infty [A(\omega)\cos\omega x + B(\omega)\sin\omega x]d\omega} \quad (2.1)$$

where  $A(\omega) = \frac{1}{\pi} \int_{-\infty}^\infty f(v)\cos(\omega v)dv$  and  $B(\omega) = \frac{1}{\pi} \int_{-\infty}^\infty f(v)\sin(\omega v)dv$ .

Substituting A and B into the integral for  $f$  (2.1), we get,

$$f(x) = \frac{1}{\pi} \int_0^\infty \int_{-\infty}^\infty f(v)[\cos(\omega v)\cos(\omega x) + \sin(\omega v)\sin(\omega x)]dvd\omega \quad (2.2)$$

Using  $\cos(a)\cos(b) + \sin(a)\sin(b) = \cos(a - b)$  in (2.2), we get

$$f(x) = \frac{1}{\pi} \int_0^\infty \left[ \int_{-\infty}^\infty f(v)\cos(\omega x - \omega v)dv \right] d\omega \quad (2.3)$$

The integral in brackets is an even function of  $\omega$ ,  $F(\omega)$ , because  $\cos(\omega x - \omega v)$  is an even function of  $\omega$ , the function  $f$  does not depend on  $\omega$ , and we integrate with respect to  $v$  not  $\omega$ . Hence the integral of  $F(\omega)$  from  $\omega = 0$  to  $\infty$  is  $\frac{1}{2}$  times the integral of  $F(\omega)$  from  $-\infty$  to  $\infty$ . Thus

$$f(x) = \frac{1}{2\pi} \int_{-\infty}^\infty \left[ \int_{-\infty}^\infty f(v)\cos(\omega x - \omega v)dv \right] d\omega \quad (2.4)$$

Since,  $\sin(\omega x - \omega v)$  is an odd function of  $\omega$ , the integral becomes an odd function of  $\omega$ , Hence

$$\frac{1}{2\pi} \int_{-\infty}^\infty \left[ \int_{-\infty}^\infty f(v)\sin(\omega x - \omega v)dv \right] d\omega = 0 \quad (2.5)$$

We now take the integrand of (2.4) plus  $\iota (= \sqrt{-1})$  times the integrand of (2.5), and use the formula  $e^{\iota x} = \cos x + \iota \sin x$ , we have

$$f(v)\cos(\omega x - \omega v) + \iota f(v)\sin(\omega x - \omega v) = f(v)e^{\iota(\omega x - \omega v)} \quad (2.6)$$

Thus, the **Complex Fourier Integral** is given by

$$\boxed{f(x) = \frac{1}{2\pi} \int_{-\infty}^\infty \int_{-\infty}^\infty f(v)e^{\iota\omega(x-v)}dvd\omega} \quad (2.7)$$

**Ques 1.** Using fourier integral representation, show that

$$\int_0^\infty \frac{\cos(\omega x) + \omega \sin(\omega x)}{1 + \omega^2} d\omega = \begin{cases} 0, & \text{if } x < 0 \\ \frac{\pi}{2}, & x = 0 \\ \pi e^{-x}, & x > 0 \end{cases}$$

**Soln.** Consider, (take  $\pi = 1$ , initially)

$$f(x) = \begin{cases} 0, & \text{if } x < 0 \\ \frac{1}{2}, & x = 0 \\ e^{-x}, & x > 0 \end{cases}$$

Consider complex form of fourier integral, (use  $e^{i\theta} = \cos\theta + i\sin\theta$ )

$$\begin{aligned} f(x) &= \frac{1}{2\pi} \int_{-\infty}^{\infty} \left[ \int_{-\infty}^{\infty} f(v) e^{-i\omega v} dv \right] e^{i\omega x} d\omega \\ &= \frac{1}{2\pi} \int_{-\infty}^{\infty} \left[ \int_{-\infty}^{\infty} e^{-v} e^{-i\omega v} dv \right] e^{i\omega x} d\omega \\ &= \frac{1}{2\pi} \int_{-\infty}^{\infty} \left[ \int_0^\infty e^{-v(1+i\omega)} dv \right] e^{i\omega x} d\omega \\ &= \frac{1}{2\pi} \int_{-\infty}^{\infty} \left[ \frac{e^{-v(1+i\omega)}}{-1-i\omega} \right] \Big|_0^\infty e^{i\omega x} d\omega \\ &= \frac{1}{2\pi} \int_{-\infty}^{\infty} \left[ \frac{1}{1+i\omega} \right] e^{i\omega x} d\omega \\ &= \frac{1}{2\pi} \int_{-\infty}^{\infty} \left[ \frac{1}{1+i\omega} \times \frac{1-i\omega}{1-i\omega} \right] (\cos\omega x + i\sin\omega x) d\omega \\ &= \frac{1}{2\pi} \int_{-\infty}^{\infty} \left[ \frac{1-i\omega}{1+\omega^2} \right] (\cos\omega x + i\sin\omega x) d\omega \\ &= \frac{1}{2\pi} \int_{-\infty}^{\infty} \left[ \frac{1}{1+\omega^2} \right] (\cos\omega x + i\sin\omega x - \omega \cos\omega x + \omega \sin\omega x) d\omega \end{aligned}$$

Considering only the real part, we get

$$= \frac{1}{\pi} \int_0^\infty \frac{\cos(\omega x) + \omega \sin(\omega x)}{1 + \omega^2} d\omega$$

Thus,

$$\frac{1}{\pi} \int_0^\infty \frac{\cos(\omega x) + \omega \sin(\omega x)}{1 + \omega^2} d\omega = \begin{cases} 0, & \text{if } x < 0 \\ \frac{1}{2}, & x = 0 \\ e^{-x}, & x > 0 \end{cases}$$

Taking  $\pi$  to the other side, we get our desired result.

### 3 Fourier Transform and its Inverse

Re-writing (2.7), as a product of exponential functions, we have

$$f(x) = \frac{1}{\sqrt{2\pi}} \int_{-\infty}^{\infty} \left[ \frac{1}{\sqrt{2\pi}} \int_{-\infty}^{\infty} f(v) e^{-i\omega v} dv \right] e^{i\omega x} d\omega \quad (3.1)$$

The expression in brackets is a function of  $\omega$ , denoted by  $\hat{f}(\omega)$ , and is called the **Fourier Transform** of  $f$ ; Re-writing  $v = x$ , we have

$$\hat{f}(\omega) = \frac{1}{\sqrt{2\pi}} \int_{-\infty}^{\infty} f(x) e^{-i\omega x} dx \quad (3.2)$$

The **Inverse Fourier Transform** of  $\hat{f}(\omega)$  is given by

$$f(x) = \frac{1}{\sqrt{2\pi}} \int_{-\infty}^{\infty} \hat{f}(\omega) e^{i\omega x} d\omega \quad (3.3)$$

Notation:

$$\hat{f} = \mathfrak{F}(f) \quad (3.4)$$

$$f = \mathfrak{F}^{-1}(\hat{f}) \quad (3.5)$$

### Result: Existence of the Fourier Transform

If  $f(x)$  is absolutely integrable on the x-axis and piecewise continuous on every finite interval, then the Fourier transform  $\hat{f}(\omega)$  of  $f(x)$  given by (3.2) exists.

### 3.1 Worked Examples

**Ques 1.** Find the Fourier Transform of  $f(x) = 1$  if  $|x| < 1$  and  $f(x) = 0$  otherwise.

**Soln.** Using  $\hat{f}(\omega) = \frac{1}{\sqrt{2\pi}} \int_{-\infty}^{\infty} f(x) e^{-i\omega x} dx$ , we get

$$\begin{aligned} \hat{f}(\omega) &= \frac{1}{\sqrt{2\pi}} \int_{-1}^1 1 \cdot e^{-i\omega x} dx \\ &= \frac{1}{\sqrt{2\pi}} \left. \frac{e^{-i\omega x}}{-i\omega} \right|_{-1}^1 \\ &= \frac{1}{-i\omega\sqrt{2\pi}} (e^{-i\omega} - e^{i\omega}) \end{aligned} \quad (3.6)$$

Using  $e^{i\omega} = \cos\omega + i\sin\omega$  and  $e^{-i\omega} = \cos\omega - i\sin\omega$ , we get,

$$e^{-i\omega} - e^{i\omega} = (\cos\omega - i\sin\omega) - (\cos\omega + i\sin\omega) = -2i\sin\omega \quad (3.7)$$

Using (3.7) in (3.6), we get

$$\begin{aligned}\hat{f}(\omega) &= \frac{1}{-\iota\omega\sqrt{2\pi}}(-2\iota\sin\omega) \\ &= \frac{2\sin\omega}{\omega\sqrt{2\pi}} \\ &= \sqrt{\frac{2}{\pi}} \frac{\sin\omega}{\omega}\end{aligned}$$

**Ques 2.** Find the Fourier Transform  $\mathfrak{F}(e^{-ax})$  of  $f(x) = e^{-ax}$  if  $x > 0$  and  $f(x) = 0$ , if  $x < 0$ , here  $a > 0$ .

**Soln.** Using  $\hat{f}(\omega) = \frac{1}{\sqrt{2\pi}} \int_{-\infty}^{\infty} f(x)e^{-\iota\omega x}dx$ , we get

$$\begin{aligned}\hat{f}(\omega) &= \frac{1}{\sqrt{2\pi}} \int_0^{\infty} e^{-ax}e^{-\iota\omega x}dx \\ &= \frac{1}{\sqrt{2\pi}} \left( \frac{e^{-(a+\iota\omega)x}}{-(a+\iota\omega)} \right) \Big|_0^{\infty} \\ &= \frac{1}{\sqrt{2\pi}} \left( \frac{1}{a+\iota\omega} \right)\end{aligned}$$

**Ques 3.** Find the Fourier Transform of  $f(x) = \begin{cases} 1, & \text{if } -b < x < b \\ 0, & \text{otherwise} \end{cases}$ .

**Soln.** Using  $\hat{f}(\omega) = \frac{1}{\sqrt{2\pi}} \int_{-\infty}^{\infty} f(x)e^{-\iota\omega x}dx$ , we get

$$\begin{aligned}\hat{f}(\omega) &= \frac{1}{\sqrt{2\pi}} \int_{-b}^b e^{-\iota\omega x}dx \\ &= \frac{1}{\sqrt{2\pi}} \frac{e^{-\iota\omega x}}{-\iota\omega} \Big|_{-b}^b \\ &= \frac{1}{\sqrt{2\pi}} \left( \frac{e^{-\iota\omega b}}{(-\iota\omega)} - \frac{e^{\iota\omega b}}{(-\iota\omega)} \right) \\ &= \frac{1}{\sqrt{2\pi}} \left( \frac{e^{-\iota\omega b}}{(-\iota\omega)} + \frac{e^{\iota\omega b}}{(\iota\omega)} \right)\end{aligned}$$

$$\hat{f}(\omega) = \frac{1}{\iota\omega\sqrt{2\pi}}(e^{\iota\omega b} - e^{-\iota\omega b})$$

Using  $\sin\theta = \frac{e^{\iota\theta} - e^{-\iota\theta}}{2\iota}$ , we get

$$\begin{aligned}\hat{f}(\omega) &= \frac{1}{\iota\omega\sqrt{2\pi}} 2\iota\sin\omega b \\ &= \sqrt{\frac{2}{\pi}} \frac{\sin b\omega}{\omega}\end{aligned}$$

**Ques 4.** Find the Fourier transform of  $f(x) = \begin{cases} e^{\iota ax}, & \text{if } -b < x < b \\ 0, & \text{otherwise} \end{cases}$ .

**Soln.** Using  $\hat{f}(\omega) = \frac{1}{\sqrt{2\pi}} \int_{-\infty}^{\infty} f(x)e^{-\iota\omega x} dx$ , we get

$$\begin{aligned} \hat{f}(\omega) &= \frac{1}{\sqrt{2\pi}} \int_{-b}^b e^{\iota ax} e^{-\iota\omega x} dx \\ &= \frac{1}{\sqrt{2\pi}} \int_{-b}^b e^{(\iota a - \iota\omega)x} dx \\ &= \frac{1}{\sqrt{2\pi}} \left. \frac{e^{(\iota a - \iota\omega)x}}{(\iota a - \iota\omega)} \right|_{-b}^b \\ &= \frac{1}{\sqrt{2\pi}} \left( \frac{e^{(\iota a - \iota\omega)b}}{(\iota a - \iota\omega)} - \frac{e^{(\iota a - \iota\omega)b}}{(\iota a - \iota\omega)} \right) \\ &= \frac{1}{\sqrt{2\pi}(\iota a - \iota\omega)} (e^{(\iota a - \iota\omega)b} - e^{-(\iota a - \iota\omega)b}) \\ &= \frac{1}{\iota\sqrt{2\pi}(a - \omega)} (e^{\iota(a-\omega)b} - e^{-\iota(a-\omega)b}) \end{aligned}$$

Using  $\sin\theta = \frac{e^{\iota\theta} - e^{-\iota\theta}}{2\iota}$ , we get

$$\begin{aligned} \hat{f}(\omega) &= \frac{1}{\iota\sqrt{2\pi}(a - \omega)} 2\iota \sin(a - \omega)b \\ &= \sqrt{\frac{2}{\pi}} \frac{\sin(a - \omega)b}{(a - \omega)} \end{aligned}$$

**Ques 5.** Find the Fourier Transform of  $e^{-|x|}$ ,  $-\infty < x < \infty$ .

**Soln.** Using  $\hat{f}(\omega) = \frac{1}{\sqrt{2\pi}} \int_{-\infty}^{\infty} f(x)e^{-\iota\omega x} dx$ , we get

$$\begin{aligned} \hat{f}(\omega) &= \frac{1}{\sqrt{2\pi}} \int_{-\infty}^{\infty} e^{-|x|} e^{-\iota\omega x} dx \\ &= \frac{1}{\sqrt{2\pi}} \int_{-\infty}^{\infty} e^{-|x|} (\cos(\omega x) - \iota \sin(\omega x)) dx \\ &= \frac{1}{\sqrt{2\pi}} \left( \int_{-\infty}^{\infty} e^{-|x|} \cos(\omega x) dx - \iota \int_{-\infty}^{\infty} e^{-|x|} \sin(\omega x) dx \right) \end{aligned}$$

The integrand  $e^{-|x|}\cos(\omega x)$  is an even function and  $e^{-|x|}\sin(\omega x)$  is an odd function; Hence  $\int_{-\infty}^{\infty} e^{-|x|}\cos(\omega x) dx = 2 \int_0^{\infty} e^{-|x|}\cos(\omega x) dx$  and  $\int_{-\infty}^{\infty} e^{-|x|}\sin(\omega x) dx = 0$ . Thus,

$$\begin{aligned} \hat{f}(\omega) &= \frac{1}{\sqrt{2\pi}} 2 \int_0^{\infty} e^{-|x|} \cos(\omega x) dx \\ &= \frac{1}{\sqrt{2\pi}} 2 \int_0^{\infty} e^{-x} \cos(\omega x) dx \end{aligned}$$

Using  $\int e^{at} \cos bt = \frac{e^{at}}{a^2 + b^2} (a \cos(bt) + b \sin(bt))$ , we get

$$\begin{aligned}\hat{f}(\omega) &= \sqrt{\frac{2}{\pi}} \left[ \frac{e^{-x}}{1 + \omega^2} (-\cos \omega x + \omega \sin \omega x) \right] \Big|_0^\infty \\ &= \sqrt{\frac{2}{\pi}} \left[ \frac{1}{1 + \omega^2} \right]\end{aligned}$$

H

**Ques 6.** Find the Fourier Transform of  $f(x) = xe^{-x}, 0 \leq x \leq \infty$ .

**Soln.** Using  $\hat{f}(\omega) = \frac{1}{\sqrt{2\pi}} \int_{-\infty}^{\infty} f(x) e^{-i\omega x} dx$ , we get

$$\begin{aligned}\hat{f}(\omega) &= \frac{1}{\sqrt{2\pi}} \int_{-\infty}^{\infty} x e^{-x} e^{-i\omega x} dx \\ &= \frac{1}{\sqrt{2\pi}} \int_0^{\infty} x e^{-x} e^{-i\omega x} dx \\ &= \frac{1}{\sqrt{2\pi}} \int_0^{\infty} x e^{-x(1+i\omega)} dx\end{aligned}$$

Using Bernoulli's rule of integration by parts,

$$\int uv = u_0 v_1 - u_1 v_2 + u_2 v_3 - u_3 v_4 + \dots$$

where  $u_0, u_1, u_2, u_3, \dots$  i.e all  $u$ 's represent successive derivatives of  $u$ ;

$v_0, v_1, v_2, v_3, \dots$  i.e all  $v$ 's represent successive integrals of  $v$ .

$$u = x, u_1 = 1, u_2 = 0, v = e^{-x(1+i\omega)}, v_1 = \frac{e^{-x(1+i\omega)}}{-(1+i\omega)}, v_2 = \frac{e^{-x(1+i\omega)}}{(1+i\omega)^2}$$

$$\begin{aligned}\hat{f}(\omega) &= \frac{1}{\sqrt{2\pi}} \left[ x \frac{e^{-x(1+i\omega)}}{-(1+i\omega)} - \frac{e^{-x(1+i\omega)}}{(1+i\omega)^2} \right] \Big|_0^\infty \\ &= \frac{1}{\sqrt{2\pi}} \left[ \frac{1}{(1+i\omega)^2} \right] \\ &= \frac{1}{\sqrt{2\pi}} \left[ \frac{1}{(1+i\omega)^2} \frac{(1-i\omega)^2}{(1-i\omega)^2} \right] \\ &= \frac{1}{\sqrt{2\pi}} \left[ \frac{(1-i\omega)^2}{(1+i\omega)^2 (1-i\omega)^2} \right] \\ &= \frac{1}{\sqrt{2\pi}} \left[ \frac{(1-i\omega)^2}{[(1+i\omega)(1-i\omega)]^2} \right] \\ &= \frac{1}{\sqrt{2\pi}} \left[ \frac{(1-i\omega)^2}{(1^2 - (i\omega)^2)^2} \right] \\ &= \frac{1}{\sqrt{2\pi}} \left[ \frac{(1-i\omega)^2}{(1 + (\omega)^2)^2} \right]\end{aligned}$$

## 4 Fourier Sine and Cosine Transform

The Fourier Transform of a function  $f(x)$  is given by

$$\widehat{f}_c(\omega) = \sqrt{\frac{2}{\pi}} \int_0^{\infty} f(x) \cos(\omega x) dx \quad (4.1)$$

The inverse Fourier Cosine Transform

$$f(x) = \sqrt{\frac{2}{\pi}} \int_0^{\infty} \widehat{f}_c(\omega) \cos(\omega x) d\omega \quad (4.2)$$

The Fourier Sine Transform is given by

$$\widehat{f}_s(\omega) = \sqrt{\frac{2}{\pi}} \int_0^{\infty} f(x) \sin(\omega x) dx \quad (4.3)$$

The inverse Fourier Sine Transform is given by

$$f(x) = \sqrt{\frac{2}{\pi}} \int_0^{\infty} \widehat{f}_s(\omega) \sin(\omega x) d\omega \quad (4.4)$$

### 4.1 Worked Examples

**Ques 1.** Find the Fourier Sine and Cosine transforms of the function

$$f(x) = \begin{cases} k, & \text{if } 0 < x < a \\ 0, & \text{if } x > a \end{cases}$$

**Soln.** Fourier sine transform of the function  $f(x)$  is given by (4.3),

$$\widehat{f}_s(\omega) = \sqrt{\frac{2}{\pi}} \int_0^{\infty} f(x) \sin(\omega x) dx, \text{ then}$$

$$\begin{aligned} \widehat{f}_s(\omega) &= \sqrt{\frac{2}{\pi}} k \int_0^a \sin(\omega x) dx \\ &= \sqrt{\frac{2}{\pi}} k \left( \frac{-\cos(\omega x)}{\omega} \right) \Big|_0^a \\ &= \sqrt{\frac{2}{\pi}} k \left( \frac{1 - \cos(\omega a)}{\omega} \right) \end{aligned}$$

Fourier cosine transform of the function  $f(x)$  is given by (4.1),

$$\widehat{f}_c(\omega) = \sqrt{\frac{2}{\pi}} \int_0^{\infty} f(x) \cos(\omega x) dx, \text{ then}$$



$$\begin{aligned}
\hat{f}_c(\omega) &= \sqrt{\frac{2}{\pi}} k \int_0^a \cos(\omega x) dx \\
&= \sqrt{\frac{2}{\pi}} k \left( \frac{\sin(\omega x)}{\omega} \right) \Big|_0^a \\
&= \sqrt{\frac{2}{\pi}} k \left( \frac{\sin(\omega a)}{\omega} \right)
\end{aligned}$$

**Ques 2.** Find the Fourier Sine and Cosine transforms of the function  $f(x) = e^{-x}$

**Soln.** Fourier cosine transform of the function  $f(x)$  is given by (4.1),

$$\hat{f}_c(\omega) = \sqrt{\frac{2}{\pi}} \int_0^\infty f(x) \cos(\omega x) dx, \text{ then}$$

$$\hat{f}_c(\omega) = \sqrt{\frac{2}{\pi}} \int_0^\infty e^{-x} \cos(\omega x) dx$$

$$\text{Using } \int e^{ax} \cos(bx) dx = \frac{e^{ax}}{a^2 + b^2} \{a \cos(bx) + b \sin(bx)\}$$

$$\begin{aligned}
\hat{f}_c(\omega) &= \sqrt{\frac{2}{\pi}} \frac{e^{-x}}{(-1)^2 + \omega^2} (-\cos(\omega x) + \omega \sin(\omega x)) \Big|_0^\infty \\
&= \sqrt{\frac{2}{\pi}} \left( \frac{1}{1 + \omega^2} \right)
\end{aligned}$$

Fourier sine transform of the function  $f(x)$  is given by (4.3),

$$\hat{f}_s(\omega) = \sqrt{\frac{2}{\pi}} \int_0^\infty f(x) \sin(\omega x) dx, \text{ then}$$

$$\hat{f}_s(\omega) = \sqrt{\frac{2}{\pi}} \int_0^\infty e^{-x} \sin(\omega x) dx$$

$$\text{Using } \int e^{ax} \sin(bx) dx = \frac{e^{ax}}{a^2 + b^2} \{a \sin(bx) - b \cos(bx)\}$$

$$\begin{aligned}
\hat{f}_s(\omega) &= \sqrt{\frac{2}{\pi}} \frac{e^{-x}}{(-1)^2 + \omega^2} (-\sin(\omega x) - \omega \cos(\omega x)) \Big|_0^\infty \\
&= \sqrt{\frac{2}{\pi}} \left( \frac{\omega}{1 + \omega^2} \right)
\end{aligned}$$

**Ques 3.** Find the Fourier sine and cosine transform of the following function

$$f(x) = \begin{cases} x, & \text{if } 0 \leq x \leq 1 \\ 2 - x, & \text{if } 1 \leq x \leq 2 \\ 0, & \text{if } x > 2 \end{cases}$$

**Soln.** Fourier cosine transform of the function  $f(x)$  is given by (4.1),

$\hat{f}_c(\omega) = \sqrt{\frac{2}{\pi}} \int_0^\infty f(x) \cos(\omega x) dx$ , then

$$\hat{f}_c(\omega) = \sqrt{\frac{2}{\pi}} \left( \int_0^1 x \cos(\omega x) dx + \int_1^2 (2-x) \cos(\omega x) dx + \int_2^\infty 0 \cdot \cos(\omega x) dx \right)$$

Using Bernoulli's rule of integration by parts,

$$\int uv = u_0 v_1 - u_1 v_2 + u_2 v_3 - u_3 v_4 + \dots$$

where  $u_0, u_1, u_2, u_3, \dots$  i.e all  $u$ 's represent successive derivatives of  $u$ ;

$v_0, v_1, v_2, v_3, \dots$  i.e all  $v$ 's represent successive integrals of  $v$ .

For  $\int_0^1 x \cos(\omega x) dx$ ,

$$u = u_0 = x, u_1 = 1, u_2 = 0 \text{ and } v = \cos(\omega x), v_1 = \frac{\sin(\omega x)}{\omega}, v_2 = -\frac{\cos(\omega x)}{\omega^2}$$

For  $\int_1^2 (2-x) \cos(\omega x) dx$ ,

$$u = u_0 = 2-x, u_1 = -1, u_2 = 0 \text{ and } v = \cos(\omega x), v_1 = \frac{\sin(\omega x)}{\omega}, v_2 = -\frac{\cos(\omega x)}{\omega^2}$$

Thus,

$$\begin{aligned} \hat{f}_c(\omega) &= \sqrt{\frac{2}{\pi}} \left[ \left( x \frac{\sin(\omega x)}{\omega} + \frac{\cos(\omega x)}{\omega^2} \right) \Big|_0^1 + \left( (2-x) \frac{\sin(\omega x)}{\omega} + \frac{\cos(\omega x)}{\omega^2} \right) \Big|_1^2 \right] \\ &= \sqrt{\frac{2}{\pi}} \left[ \left( \frac{\sin(\omega)}{\omega} + \frac{\cos(\omega)}{\omega^2} - \frac{1}{\omega^2} \right) + \left( -\frac{\cos(2\omega)}{\omega^2} - \frac{\sin(\omega)}{\omega} + \frac{\cos(\omega)}{\omega^2} \right) \right] \\ &= \sqrt{\frac{2}{\pi}} \left( \frac{2\cos(\omega) - 1 - \cos(2\omega)}{\omega^2} \right) \\ &= \sqrt{\frac{2}{\pi}} \left( \frac{2\cos(\omega) - (1 + \cos(2\omega))}{\omega^2} \right), \quad \text{Using } 1 + \cos(2\omega) = 2\cos^2\omega \\ &= \sqrt{\frac{2}{\pi}} \left( \frac{2\cos(\omega) - 2\cos^2(\omega)}{\omega^2} \right) \\ &= \sqrt{\frac{2}{\pi}} \left( \frac{2\cos(\omega)(1 - \cos(\omega))}{\omega^2} \right) \end{aligned}$$

Fourier sine transform of the function  $f(x)$  is given by (4.1),

$\hat{f}_s(\omega) = \sqrt{\frac{2}{\pi}} \int_0^\infty f(x) \sin(\omega x) dx$ , then

$$\hat{f}_s(\omega) = \sqrt{\frac{2}{\pi}} \left( \int_0^1 x \sin(\omega x) dx + \int_1^2 (2-x) \sin(\omega x) dx + \int_2^\infty 0 \cdot \sin(\omega x) dx \right)$$

Using Bernoulli's rule of integration by parts,

$$\int uv = u_0 v_1 - u_1 v_2 + u_2 v_3 - u_3 v_4 + \dots$$

where  $u_0, u_1, u_2, u_3, \dots$  i.e all  $u$ 's represent successive derivatives of  $u$ ;

$v_0, v_1, v_2, v_3, \dots$  i.e all  $v$ 's represent successive integrals of  $v$ .

For  $\int_0^1 x \sin(\omega x) dx$ ,  
 $u = u_0 = x, u_1 = 1, u_2 = 0$  and  $v = \sin(\omega x), v_1 = \frac{-\cos(\omega x)}{\omega}, v_2 = \frac{-\sin(\omega x)}{\omega^2}$

For  $\int_1^2 (2-x) \sin(\omega x) dx$ ,  
 $u = u_0 = 2-x, u_1 = -1, u_2 = 0$  and  $v = \sin(\omega x), v_1 = \frac{-\cos(\omega x)}{\omega}, v_2 = \frac{-\sin(\omega x)}{\omega^2}$

Thus,

$$\begin{aligned}\hat{f}_c(\omega) &= \sqrt{\frac{2}{\pi}} \left[ \left( -x \frac{\cos(\omega x)}{\omega} + \frac{\sin(\omega x)}{\omega^2} \right) \Big|_0^1 + \left( -(2-x) \frac{\cos(\omega x)}{\omega} - \frac{\sin(\omega x)}{\omega^2} \right) \Big|_1^2 \right] \\ &= \sqrt{\frac{2}{\pi}} \left[ \left( \frac{-\cos(\omega)}{\omega} + \frac{\sin(\omega)}{\omega^2} \right) + \left( -\frac{\sin(2\omega)}{\omega^2} + \frac{\cos(\omega)}{\omega} + \frac{\sin(\omega)}{\omega^2} \right) \right] \\ &= \sqrt{\frac{2}{\pi}} \left( \frac{2\sin(\omega) - \sin(2\omega)}{\omega^2} \right) \\ &= \sqrt{\frac{2}{\pi}} \left( \frac{2\sin(\omega) - 2\sin(\omega)\cos(\omega)}{\omega^2} \right), \quad \text{Using } \sin(2\omega) = 2\sin(\omega)\cos(\omega) \\ &= \sqrt{\frac{2}{\pi}} \left( \frac{2\sin(\omega)(1 - \cos(\omega))}{\omega^2} \right)\end{aligned}$$

**Ques 4.** Find the Fourier cosine transform of the function

$$f(x) = \begin{cases} \cos(x), & \text{if } 0 < x < a \\ 0, & \text{if } x \geq a \end{cases}$$

**Soln.** Fourier cosine transform of the function  $f(x)$  is given by (4.1),

$$\hat{f}_c(\omega) = \sqrt{\frac{2}{\pi}} \int_0^\infty f(x) \cos(\omega x) dx, \text{ then}$$

$$\hat{f}_c(\omega) = \sqrt{\frac{2}{\pi}} \int_0^a \cos(x) \cos(\omega x) dx$$

Using  $\cos(a)\cos(b) = \frac{1}{2} (\cos(a+b) + \cos(a-b))$ ,

$$\begin{aligned}\hat{f}_c(\omega) &= \sqrt{\frac{2}{\pi}} \int_0^a \frac{1}{2} (\cos(1+\omega)x + \cos(1-\omega)x) dx \\ &= \frac{1}{\sqrt{2\pi}} \left( \frac{\sin(1+\omega)x}{1+\omega} + \frac{\sin(1-\omega)x}{1-\omega} \right) \Big|_0^a \\ &= \frac{1}{\sqrt{2\pi}} \left( \frac{\sin(1+\omega)a}{1+\omega} + \frac{\sin(1-\omega)a}{1-\omega} \right)\end{aligned}$$